lseq as nat to intytypes

code/ecdsa/Hacl.Spec.EC.Definition.fst
@@ -7,6 +7,7 @@ open Lib.Sequence
 open FStar.Mul
 
 open Spec.ECC.Curves
+open FStar.Math.Lemmas
 
 #set-options " --z3rlimit 100"
 
@@ -72,7 +73,8 @@ val lemma_create_zero_buffer: len: size_nat {len > 0} -> c: curve -> Lemma (lseq
 let lemma_create_zero_buffer len c = lemma_create_ #len len
 
 
-val lemma_lseq_as_seq_as_forall: #l: size_nat -> a: lseq uint64 l -> b: lseq uint64 l -> i: nat {i >= 0 /\ i <= l} ->
+val lemma_lseq_as_seq_as_forall: #l: size_nat -> #t:inttype{unsigned t}
+  -> a: lseq (uint_t t SEC) l -> b: lseq (uint_t t SEC) l -> i: nat {i >= 0 /\ i <= l} ->
   Lemma ((forall (k: nat). k <= (i - 1) ==> Lib.Sequence.index a k == Lib.Sequence.index b k) ==>
     (lseq_as_nat_ #l a i == lseq_as_nat_ #l b i))
 
@@ -85,16 +87,16 @@ let rec lemma_lseq_as_seq_as_forall #l a b i =
     lseq_as_nat_definiton b i
     
 
-val lemma_lseq_1: l: size_nat -> a: lseq uint64 l -> i: nat {i > 0 /\ i <= l} ->
-  Lemma (lseq_as_nat_ a i % pow2 64 == v (Lib.Sequence.index a 0))
+val lemma_lseq_1: #l: size_nat -> #t:inttype{unsigned t} -> a: lseq (uint_t t SEC) l  -> i: nat {i > 0 /\ i <= l} ->
+  Lemma (lseq_as_nat_ a i % pow2 (bits t) == v (Lib.Sequence.index a 0))
 
-let rec lemma_lseq_1 l a i = 
+let rec lemma_lseq_1 #l #t a i = 
   match i with 
   |1 -> ()
-  |_ -> lemma_lseq_1 l a (i - 1);
+  |_ -> lemma_lseq_1 #l a (i - 1);
     lseq_as_nat_definiton a i;
-    FStar.Math.Lemmas.lemma_mod_add_distr (lseq_as_nat_ a (i - 1)) (pow2 (64 * (i - 1)) * v (Lib.Sequence.index a (i - 1))) (pow2 64);
-    FStar.Math.Lemmas.pow2_multiplication_modulo_lemma_1 (v (Lib.Sequence.index a (i - 1))) 64 (64 * (i - 1))  
+    FStar.Math.Lemmas.lemma_mod_add_distr (lseq_as_nat_ a (i - 1)) (pow2 (bits t * (i - 1)) * v (Lib.Sequence.index a (i - 1))) (pow2 (bits t));
+    FStar.Math.Lemmas.pow2_multiplication_modulo_lemma_1 (v (Lib.Sequence.index a (i - 1))) (bits t) ((bits t) * (i - 1))  
 
 
 val lemma_lseq_as_seq_extension: 
@@ -123,21 +125,27 @@ let rec lemma_lseq_as_seq_extension #l0 #l1 a0 a1 i =
     assert (Lib.Sequence.index a0 (i - 1) == Lib.Sequence.index a1 (i - 1))
 
 
-val lseq_upperbound_: #len:size_nat -> a: lseq uint64 len -> i: nat {i >= 0 /\ i <= len} -> Lemma (lseq_as_nat_ a i < pow2 (64 * i))
+#push-options "--z3rlimit 200"
 
-let rec lseq_upperbound_ #len a i = 
+val lseq_upperbound_: #len:size_nat -> #t:inttype{unsigned t} -> a: lseq (uint_t t SEC) len -> i: nat {i >= 0 /\ i <= len} -> 
+  Lemma (lseq_as_nat_ a i < pow2 (bits t * i))
+
+let rec lseq_upperbound_ #len #t a i = 
   match i with 
   |0 -> ()
   |_ -> lseq_upperbound_ a (i - 1); 
-    lseq_as_nat_definiton a i;
-    FStar.Math.Lemmas.pow2_plus 64 (64 * (i - 1))
+    lseq_as_nat_definiton a i; 
+    FStar.Math.Lemmas.lemma_mult_le_left (pow2 (bits t * (i - 1))) (v (index a (i - 1))) (pow2 (bits t) - 1);
+    FStar.Math.Lemmas.pow2_plus (bits t) (bits t * (i - 1))
 
-val lseq_upperbound: #l: size_nat -> a: lseq uint64 l -> Lemma (lseq_as_nat a < pow2 (64 * l))
+
+val lseq_upperbound: #l: size_nat -> #t:inttype{unsigned t} -> a: lseq (uint_t t SEC) l 
+  -> Lemma (lseq_as_nat a < pow2 (bits t * l))
 
 let lseq_upperbound #l a = lseq_upperbound_  a l
 
 
-val lseq_upperbound2: #l: size_nat -> a: lseq uint64 l -> i: nat {i >= 0 /\ i <= l} -> 
+val lseq_upperbound2: #l: size_nat -> #t:inttype{unsigned t} -> a: lseq (uint_t t SEC) l -> i: nat {i >= 0 /\ i <= l} -> 
   Lemma (lseq_as_nat_ a (l - i) <= lseq_as_nat a)
 
 let rec lseq_upperbound2 #l a i = 
@@ -146,29 +154,31 @@ let rec lseq_upperbound2 #l a i =
   |_ -> lseq_upperbound2 #l a (i - 1); lseq_as_nat_definiton a (l - 1 + 1)
 
 
-val lseq_upperbound1: #l: size_nat -> a: lseq uint64 l -> i: nat {i > 0 /\ i < l} -> k: nat{k >= 0 && k <= l - i} -> Lemma 
-  (requires lseq_as_nat a < pow2 (64 * i))
+val lseq_upperbound1: #l: size_nat -> #t:inttype{unsigned t} -> a: lseq (uint_t t SEC) l -> i: nat {i > 0 /\ i < l} 
+  -> k: nat{k >= 0 && k <= l - i} -> Lemma 
+  (requires lseq_as_nat a < pow2 (bits t * i))
   (ensures lseq_as_nat_ a i == lseq_as_nat_ a (i + k))
 
-let rec lseq_upperbound1 #l a i k = 
+let rec lseq_upperbound1 #l #t a i k = 
   match k with 
   |0 -> ()
   |_ -> lseq_upperbound1 #l a i (k - 1);
     lseq_as_nat_definiton a (i + 1); 
     lseq_upperbound2 a (l - i - k);
     if (v (Lib.Sequence.index a (i + k - 1)) >= 1) then begin
-      assert(pow2 (64 * (i + k - 1)) <= pow2 (64 * (i + k - 1)) * v (Lib.Sequence.index a (i + k - 1)));
-      assert((64 * i) <= 64 * (i + k - 1));
-      FStar.Math.Lemmas.pow2_le_compat (64 * (i + k - 1)) (64 * i);
+      assert(pow2 (bits t * (i + k - 1)) <= pow2 (bits t * (i + k - 1)) * v (Lib.Sequence.index a (i + k - 1)));
+      assert((bits t * i) <= bits t * (i + k - 1));
+      FStar.Math.Lemmas.pow2_le_compat (bits t * (i + k - 1)) (bits t * i);
       assert(False)
   end
 
 
-val lemma_lseq_as_seq_as_forall_r_: #l: size_nat -> a: lseq uint64 l -> b: lseq uint64 l -> i: nat {i >= 1 /\ i <= l} -> 
+val lemma_lseq_as_seq_as_forall_r_: #l: size_nat -> #t:inttype{unsigned t} 
+  -> a: lseq (uint_t t SEC) l -> b: lseq (uint_t t SEC) l -> i: nat {i >= 1 /\ i <= l} -> 
   Lemma (requires lseq_as_nat_ a i == lseq_as_nat_ #l b i)
   (ensures lseq_as_nat_ a (i - 1) == lseq_as_nat_ #l b (i - 1))
 
-let lemma_lseq_as_seq_as_forall_r_ #l a b i = 
+let lemma_lseq_as_seq_as_forall_r_ #l #t a b i = 
   lseq_as_nat_definiton a i;
   lseq_as_nat_definiton b i;
   
@@ -178,34 +188,53 @@ let lemma_lseq_as_seq_as_forall_r_ #l a b i =
   let ai = v (Lib.Sequence.index a (i - 1)) in 
   let bi = v (Lib.Sequence.index b (i - 1)) in 
 
-  FStar.Math.Lemmas.lemma_mod_plus (lseq_as_nat_ a (i - 1)) ai (pow2 (64 * (i - 1)));
-  FStar.Math.Lemmas.lemma_mod_plus (lseq_as_nat_ b (i - 1)) bi (pow2 (64 * (i - 1)));
+  FStar.Math.Lemmas.lemma_mod_plus (lseq_as_nat_ a (i - 1)) ai (pow2 (bits t * (i - 1)));
+  FStar.Math.Lemmas.lemma_mod_plus (lseq_as_nat_ b (i - 1)) bi (pow2 (bits t * (i - 1)));
 
   let open FStar.Tactics in 
   let open FStar.Tactics.Canon in 
 
-  assert_by_tactic (ai * pow2 (64 * (i - 1)) == pow2 (64 * (i - 1)) * ai) canon;
-  assert_by_tactic (bi * pow2 (64 * (i - 1)) == pow2 (64 * (i - 1)) * bi) canon;
+  assert_by_tactic (ai * pow2 (bits t * (i - 1)) == pow2 (bits t * (i - 1)) * ai) canon;
+  assert_by_tactic (bi * pow2 (bits t * (i - 1)) == pow2 (bits t * (i - 1)) * bi) canon;
 
-  FStar.Math.Lemmas.small_mod (lseq_as_nat_ a (i - 1)) (pow2 (64 * (i - 1)));
-  FStar.Math.Lemmas.small_mod (lseq_as_nat_ b (i - 1)) (pow2 (64 * (i - 1)))
+  FStar.Math.Lemmas.small_mod (lseq_as_nat_ a (i - 1)) (pow2 (bits t * (i - 1)));
+  FStar.Math.Lemmas.small_mod (lseq_as_nat_ b (i - 1)) (pow2 (bits t * (i - 1)))
 
+#push-options "--z3rlimit 300"
 
-val lemma_lseq_as_seq_as_forall_r: #l: size_nat -> a: lseq uint64 l -> b: lseq uint64 l -> i: nat {i >= 0 /\ i <= l} ->
-  Lemma ((lseq_as_nat_ #l a i == lseq_as_nat_ #l b i) ==> (forall (k: nat). k <= (i - 1) ==> Lib.Sequence.index a k == Lib.Sequence.index b k))
+val lemma_lseq_as_seq_as_forall_r: #l: size_nat -> #t:inttype{unsigned t} 
+  -> a: lseq (uint_t t SEC) l -> b: lseq (uint_t t SEC) l -> i: nat {i >= 0 /\ i <= l} ->
+  Lemma ((lseq_as_nat_ #l a i == lseq_as_nat_ #l b i) 
+    ==> (forall (k: nat). k <= (i - 1) ==> Lib.Sequence.index a k == Lib.Sequence.index b k))
 
-let rec lemma_lseq_as_seq_as_forall_r #l a b i = 
+let rec lemma_lseq_as_seq_as_forall_r #l #t a b i = 
   match i with 
   |0 -> ()
-  |_ -> lemma_lseq_as_seq_as_forall_r #l a b (i - 1);
+  |_ -> 
+    lemma_lseq_as_seq_as_forall_r #l a b (i - 1);
     let i_1 = i - 1 in 
+
     lseq_as_nat_definiton a i;
     lseq_as_nat_definiton b i;
-    if lseq_as_nat_ a i = lseq_as_nat_ b i then
-      lemma_lseq_as_seq_as_forall_r_ a b i
+    if lseq_as_nat_ a i = lseq_as_nat_ b i then lemma_lseq_as_seq_as_forall_r_ a b i;
+
+    let ai = v (index a (i - 1)) in 
+    let bi = v (index b (i - 1)) in 
+    let p = pow2 (bits t * (i - 1)) in 
+
+    let open FStar.Tactics.Canon in 
+    let open FStar.Tactics in 
+
+    assert_by_tactic (p * ai == ai * p) canon;
+    assert_by_tactic (p * bi == bi * p) canon;
+    
+    assert(lseq_as_nat_ a i == lseq_as_nat_ b i ==> ai * pow2 (bits t * (i - 1)) == bi * pow2 (bits t * (i - 1)));
+
+    if ai * p = bi * p then lemma_cancel_mul ai bi p
 
 
-val lemma_lseq_as_seq_as_forall_lr: #l: size_nat -> a: lseq uint64 l -> b: lseq uint64 l -> i: nat {i >= 0 /\ i <= l} -> 
+val lemma_lseq_as_seq_as_forall_lr: #l: size_nat -> #t:inttype{unsigned t} 
+  -> a: lseq (uint_t t SEC) l -> b: lseq (uint_t t SEC) l -> i: nat {i >= 0 /\ i <= l} -> 
   Lemma ((lseq_as_nat_ #l a i == lseq_as_nat_ #l b i) <==> (forall (k: nat). k <= (i - 1) ==> Lib.Sequence.index a k == Lib.Sequence.index b k))
 
 let lemma_lseq_as_seq_as_forall_lr #l a b i = 
@@ -213,7 +242,8 @@ let lemma_lseq_as_seq_as_forall_lr #l a b i =
   lemma_lseq_as_seq_as_forall_r #l a b i
 
 
-val lseq_as_nat_zero_l: #l: size_nat -> a: lseq uint64 l -> i: nat {i >= 0 /\ i <= l} -> Lemma 
+val lseq_as_nat_zero_l:  #l: size_nat -> #t:inttype{unsigned t} 
+  -> a: lseq (uint_t t SEC) l  -> i: nat {i >= 0 /\ i <= l} -> Lemma 
   (lseq_as_nat_ a i == 0 ==> (forall (j: nat {j < i}). v (Lib.Sequence.index a j) == 0))
 
 let rec lseq_as_nat_zero_l #l a i = 
@@ -222,7 +252,8 @@ let rec lseq_as_nat_zero_l #l a i =
   |_ -> lseq_as_nat_zero_l #l a (i - 1); lseq_as_nat_definiton a i
 
 
-val lseq_as_nat_zero_r: #l: size_nat -> a: lseq uint64 l -> i: nat {i >= 0 /\ i <= l} -> Lemma 
+val lseq_as_nat_zero_r:  #l: size_nat -> #t:inttype{unsigned t} 
+  -> a: lseq (uint_t t SEC) l  -> i: nat {i >= 0 /\ i <= l} -> Lemma 
   ((forall (j: nat {j < i}). v (Lib.Sequence.index a j) == 0) ==> lseq_as_nat_ a i == 0)
 
 let rec lseq_as_nat_zero_r #l a i = 
@@ -231,15 +262,14 @@ let rec lseq_as_nat_zero_r #l a i =
   |_ -> lseq_as_nat_zero_r #l a (i - 1); lseq_as_nat_definiton a i
 
 
-val lseq_as_nat_zero: #l: size_nat -> a: lseq uint64 l -> Lemma 
+val lseq_as_nat_zero:  #l: size_nat -> #t:inttype{unsigned t} -> a: lseq (uint_t t SEC) l  -> Lemma 
   (lseq_as_nat_ a l == 0 <==> (forall (j: nat {j < l}). v (Lib.Sequence.index a j) == 0))
 
 let lseq_as_nat_zero #l a = 
   lseq_as_nat_zero_l #l a l;
   lseq_as_nat_zero_r #l a l
 
-
-#push-options " --z3rlimit 200 --max_fuel 0 --max_ifuel 0"
+#push-options " --z3rlimit 100 --max_fuel 0 --max_ifuel 0"
 
 val lemma_test_: #l: size_nat -> #t:inttype{unsigned t} -> a: lseq (uint_t t SEC) l -> i: nat {i <> 0 /\ i < l} -> 
   Lemma
@@ -325,6 +355,7 @@ let rec lemma_test #l #t a i =
       }
     end end
 
+#pop-options
 
 val lemma_lseq_as_bn_v_: #l: size_nat -> a: Lib.Sequence.lseq uint64 l -> i: nat{i <= l} ->
   Lemma (lseq_as_nat_ #l a i == Hacl.Spec.Bignum.Definitions.eval_ l a i) 
